Network_Security_Policy_Verification/Examples/Example_Forte14.thy
@@ -1,5 +1,5 @@
 theory Example_Forte14
-imports "../Impl_List_Interface"
+imports "../TopoS_Impl"
 begin
 
 
